RTLgenproof, RTLmachproof, Renumberproof

backend/RTLgenproof.v
@@ -724,33 +724,19 @@ Proof.
   exploit external_call_mem_extends; eauto.
   eapply Mem.push_stage_extends; eauto.
   intros [v' [tm2 [A [B [C D]]]]].
-<<<<<<< HEAD
   rewrite <- Genv.find_funct_find_funct_ptr in H0.
+  edestruct Mem.pop_stage_extends as (tm2' & USB & EXT'). apply C. apply Mem.pop_push_stage.
   exploit functions_translated; eauto. simpl. intros [tf [P Q]]. inv Q.
-  exists (rs1#rd <- v'); exists tm2.
-=======
-  edestruct Mem.pop_stage_extends as (tm2' & USB & EXT'). apply C.
-  apply Mem.pop_push_stage.
-  exploit function_ptr_translated; eauto. simpl. intros [tf [P Q]]. inv Q.
-  exists (rs1#rd <- v'); exists tm2'.
->>>>>>> origin/StackAware-new
+  exists (rs1#rd <- v'), tm2'.
 (* Exec *)
   exploit (functions_translated (Vptr b Ptrofs.zero)); eauto. cbn.
   destruct Ptrofs.eq_dec; try congruence. intros (tf & TFIND & TF). inv TF.
   split. eapply star_trans. eexact EX1.
-<<<<<<< HEAD
-  eapply star_left. eapply exec_Icall; eauto.
+  eapply star_left. eapply exec_Icall; eauto. reflexivity.
   cbn. unfold Genv.symbol_address. cbn in H. rewrite H. eauto. auto.
   eapply star_left. eapply exec_function_external.
   cbn. unfold Genv.symbol_address. cbn in H. rewrite H. eauto. eauto.
-  apply star_one. apply exec_return.
-=======
-  eapply star_left. eapply exec_Icall; eauto. reflexivity.
-  simpl. rewrite symbols_preserved. rewrite H. eauto. auto.
-  eapply star_left. eapply exec_function_external.
-  eapply external_call_symbols_preserved; eauto. apply senv_preserved.
   apply star_one. apply exec_return. eauto.
->>>>>>> origin/StackAware-new
   reflexivity. reflexivity. reflexivity.
 (* Match-env *)
   split. eauto with rtlg.
@@ -1017,15 +1003,9 @@ Lemma invert_eval_builtin_arg:
   /\ Events.eval_builtin_arg ge (fun v => v) sp m (fst (convert_builtin_arg a vl)) v
   /\ (forall vl', convert_builtin_arg a (vl ++ vl') = (fst (convert_builtin_arg a vl), vl')).
 Proof.
-<<<<<<< HEAD
   induction 1; simpl. 2-8: try (econstructor; intuition eauto with evalexpr barg; fail).
 - econstructor; split; eauto with evalexpr. split. constructor. auto. 
 - econstructor; split; eauto with evalexpr. split. repeat constructor. auto.
-=======
-  induction 1; simpl; try (econstructor; intuition eauto with evalexpr barg; fail).
-- econstructor; split; eauto with evalexpr. split. constructor. auto.
-- econstructor; split; eauto with evalexpr. split. constructor. auto.
->>>>>>> origin/StackAware-new
 - econstructor; split; eauto with evalexpr. split. repeat constructor. auto.
 - destruct IHeval_builtin_arg1 as (vl1 & A1 & B1 & C1).
   destruct IHeval_builtin_arg2 as (vl2 & A2 & B2 & C2).
@@ -1241,23 +1221,13 @@ Inductive match_states: CminorSel.state -> RTL.state -> Prop :=
       match_states (CminorSel.State f s k sp e m)
                    (RTL.State cs tf sp ns rs tm)
   | match_callstate:
-<<<<<<< HEAD
-      forall vf args targs k m tm cs tvf
-=======
-      forall f args targs k m tm cs tf id
-        (TF: transl_fundef f = OK tf)
->>>>>>> origin/StackAware-new
+      forall vf args targs k m tm cs tvf id
         (MS: match_stacks k cs)
         (LF: Val.lessdef vf tvf)
         (LD: Val.lessdef_list args targs)
         (MEXT: Mem.extends m tm),
-<<<<<<< HEAD
-      match_states (CminorSel.Callstate vf args k m)
-                   (RTL.Callstate cs tvf targs tm)
-=======
-      match_states (CminorSel.Callstate f args k m id)
-                   (RTL.Callstate cs tf targs tm id)
->>>>>>> origin/StackAware-new
+      match_states (CminorSel.Callstate vf args k m id)
+                   (RTL.Callstate cs tvf targs tm id)
   | match_returnstate:
       forall v tv k m tm cs
         (MS: match_stacks k cs)
@@ -1385,42 +1355,28 @@ Proof.
   exploit functions_translated; eauto. intros [tf' [P Q]].
   econstructor; split.
   left; eapply plus_right. eapply star_trans. eexact A. eexact E. reflexivity.
-<<<<<<< HEAD
-  eapply exec_Icall; eauto. simpl. rewrite J. eauto. simpl; auto.
-  apply sig_transl_function; auto.
-  traceEq.
-  constructor; auto. econstructor; eauto.
-  simpl. rewrite J. eauto. simpl; auto.
-=======
-  eapply exec_Icall; eauto. simpl. rewrite J. rewrite <- H3. auto. left. auto.
+  eapply exec_Icall; eauto.
+  simpl. rewrite J. rewrite <- H3. auto. left. auto.
   simpl. rewrite J. rewrite <- H3. eauto. left. auto.
   apply sig_transl_function; auto.
   traceEq.
-  constructor; auto. econstructor; eauto. eapply Mem.push_stage_extends; eauto.
->>>>>>> origin/StackAware-new
+  constructor; auto. econstructor; eauto.
+  simpl. rewrite J. rewrite <- H3. eauto. left. auto.
+  eapply Mem.push_stage_extends. eauto.
   (* direct *)
   exploit transl_exprlist_correct; eauto.
   intros [rs'' [tm'' [E [F [G [J Y]]]]]].
   exploit functions_translated; eauto. intros [tf' [P Q]].
   econstructor; split.
   left; eapply plus_right. eexact E.
-<<<<<<< HEAD
-  eapply exec_Icall; eauto. simpl.
-    unfold Genv.symbol_address. cbn in H4. rewrite H4. eauto.
-=======
   eapply exec_Icall; eauto. simpl. reflexivity. simpl.
-  rewrite symbols_preserved. rewrite H5.
-    rewrite Genv.find_funct_find_funct_ptr in P. eauto.
->>>>>>> origin/StackAware-new
+    unfold Genv.symbol_address. cbn in H5. rewrite H5. eauto.
   apply sig_transl_function; auto.
   traceEq.
   apply Genv.genv_vars_eq in H5 as H6. inv H6.
   constructor; auto. econstructor; eauto.
-<<<<<<< HEAD
-  cbn. unfold Genv.symbol_address. cbn in H4. rewrite H4. auto.
-=======
-  eapply Mem.push_stage_extends; eauto.
->>>>>>> origin/StackAware-new
+  cbn. unfold Genv.symbol_address. cbn in H5. rewrite H5. auto.
+  eapply Mem.push_stage_extends. eauto.
 
   (* tailcall *)
   inv TS; inv H0.
@@ -1432,51 +1388,35 @@ Proof.
   exploit functions_translated; eauto. intros [tf' [P Q]].
   exploit match_stacks_call_cont; eauto. intros [U V].
   assert (fn_stacksize tf = fn_stackspace f). inv TF; auto.
-<<<<<<< HEAD
   edestruct Mem.free_parallel_extends as [tm''' [ ]]; eauto.
-  econstructor; split.
-  left; eapply plus_right. eapply star_trans. eexact A. eexact E. reflexivity.
-  eapply exec_Itailcall; eauto. simpl. rewrite J. eauto. simpl; auto.
-=======
-  edestruct Mem.free_parallel_extends as [tm''' []]; eauto.
   inversion H8. rewrite mext_sup in H5.
   econstructor; split.
   left; eapply plus_right. eapply star_trans. eexact A. eexact E. reflexivity.
-  eapply exec_Itailcall; eauto. simpl. rewrite J. rewrite H3. auto. left. auto.
+  eapply exec_Itailcall; eauto. simpl. rewrite J. eauto. simpl; auto.
   simpl. rewrite J. rewrite <- H3. eauto. left. auto.
->>>>>>> origin/StackAware-new
   apply sig_transl_function; auto.
   rewrite H; eauto.
   traceEq.
   constructor; auto.
-  simpl. rewrite J. eauto. simpl; auto.
+  simpl. rewrite J. rewrite <- H3. eauto. simpl; auto.
   (* direct *)
   exploit transl_exprlist_correct; eauto.
   intros [rs'' [tm'' [E [F [G [J Y]]]]]].
   exploit functions_translated; eauto. intros [tf' [P Q]].
   exploit match_stacks_call_cont; eauto. intros [U V].
   assert (fn_stacksize tf = fn_stackspace f). inv TF; auto.
-<<<<<<< HEAD
   edestruct Mem.free_parallel_extends as [tm''' [ ]]; eauto.
-  econstructor; split.
-  left; eapply plus_right. eexact E.
-  eapply exec_Itailcall; eauto.
-  simpl. unfold Genv.symbol_address. cbn in H5. rewrite H5. eauto.
-=======
-  edestruct Mem.free_parallel_extends as [tm''' []]; eauto.
   inversion H3. rewrite mext_sup in H5.
   econstructor; split.
   left; eapply plus_right. eexact E.
-  eapply exec_Itailcall; eauto. simpl. reflexivity. simpl.
-  rewrite symbols_preserved. rewrite H7.
-  rewrite Genv.find_funct_find_funct_ptr in P. eauto.
->>>>>>> origin/StackAware-new
+  eapply exec_Itailcall; eauto. simpl. reflexivity.
+  simpl. unfold Genv.symbol_address. cbn in H7. rewrite H7. eauto.
   apply sig_transl_function; auto.
   rewrite H; eauto.
   traceEq.
-  apply Genv.genv_vars_eq in H7. inv H7.
+  apply Genv.genv_vars_eq in H7 as EQ. inv EQ.
   constructor; auto.
-  simpl. unfold Genv.symbol_address. cbn in H5. rewrite H5. eauto.
+  simpl. unfold Genv.symbol_address. cbn in H7. rewrite H7. eauto.
 
   (* builtin *)
   inv TS.
@@ -1493,13 +1433,7 @@ Proof.
   exploit Mem.pop_stage_extends; eauto. intros (tm''' & A' & B').
   econstructor; split.
   left. eapply plus_right. eexact E.
-<<<<<<< HEAD
   eapply exec_Ibuiltin; eauto.
-=======
-  eapply exec_Ibuiltin. eauto.
-  eapply eval_builtin_args_preserved with (ge1 := ge); eauto. exact symbols_preserved.
-  eapply external_call_symbols_preserved. apply senv_preserved. eauto. eauto.
->>>>>>> origin/StackAware-new
   traceEq.
   econstructor; eauto. constructor.
   eapply match_env_update_res; eauto.
@@ -1605,12 +1539,8 @@ Proof.
     assert (map_valid init_mapping s0) by apply init_mapping_valid.
     exploit (add_vars_valid (CminorSel.fn_params f)); eauto. intros [A B].
     eapply add_vars_wf; eauto. eapply add_vars_wf; eauto. apply init_mapping_wf.
-<<<<<<< HEAD
   edestruct Mem.alloc_extends as [tm' [ ]]; eauto; try apply Z.le_refl.
-=======
-  edestruct Mem.alloc_extends as [tm' []]; eauto; try apply Z.le_refl.
-  edestruct Mem.record_frame_extends as [tm'' []]; eauto.
->>>>>>> origin/StackAware-new
+  edestruct Mem.record_frame_extends as [tm'' [ ]]; eauto.
   econstructor; split.
   left; apply plus_one. eapply exec_function_internal; simpl; eauto.
   simpl. econstructor; eauto.
@@ -1627,7 +1557,7 @@ Proof.
 
   (* return *)
   inv MS.
-  edestruct Mem.pop_stage_extends as [tm' []]; eauto.
+  edestruct Mem.pop_stage_extends as [tm' [ ]]; eauto.
   econstructor; split.
   left; apply plus_one; constructor. eauto.
   econstructor; eauto. constructor.
@@ -1641,21 +1571,10 @@ Proof.
   intros. inv H0. inv H. uncklr.
   exploit functions_translated; eauto. intros [tf [A B]].
   setoid_rewrite <- (sig_transl_function (Internal f)); eauto.
-  monadInv B.
+  monadInv B. inv H5.
   econstructor; split.
-<<<<<<< HEAD
   - econstructor; eauto.
-  - econstructor; eauto. constructor.
-=======
-  econstructor. apply (Genv.init_mem_transf_partial TRANSL); eauto.
-  replace (prog_main tprog) with (prog_main prog). rewrite symbols_preserved; eauto.
-  symmetry; eapply match_program_main; eauto.
-  eexact A.
-  rewrite <- H2. apply sig_transl_function; auto. eauto.
-  setoid_rewrite (match_program_main TRANSL).
-  constructor. auto. constructor.
-  constructor. apply Mem.extends_refl.
->>>>>>> origin/StackAware-new
+  - econstructor; eauto. constructor. apply Mem.push_stage_extends. auto.
 Qed.
 
 Lemma transl_final_states:
@@ -1663,38 +1582,32 @@ Lemma transl_final_states:
   exists r2, RTL.final_state R r2 /\ match_reply (cc_c ext) w r1 r2.
 Proof.
   intros. inv H0. inv H. inv MS.
-  eexists; split. constructor; auto.
+  exploit Mem.pop_stage_extends; eauto. intros (m'' & POP' & EXT').
+  eexists; split. constructor; eauto.
   exists tt. split; constructor; uncklr; auto.
 Qed.
 
-<<<<<<< HEAD
 Lemma transl_external_states:
   forall S R q1, match_states S R -> CminorSel.at_external ge S q1 ->
   exists q2, RTL.at_external tge R q2 /\ match_query (cc_c ext) tt q1 q2 /\ se = se /\
   forall r1 r2 S', match_reply (cc_c ext) tt r1 r2 -> CminorSel.after_external S r1 S' ->
   exists R', RTL.after_external R r2 R' /\ match_states S' R'.
-=======
-Theorem transf_program_correct:
-  forward_simulation (CminorSel.semantics fn_stack_requirements prog)
-                     (RTL.semantics fn_stack_requirements tprog).
->>>>>>> origin/StackAware-new
 Proof.
   intros. inv H0. inv H.
   exploit functions_translated; eauto. intros [tf' [P TF]].
-  monadInv TF.
+  monadInv TF. inv LF.
   eexists; intuition idtac.
   - econstructor; eauto.
-  - destruct LF; try discriminate. econstructor; uncklr; eauto.
-    destruct v; cbn in *; congruence.
-  - inv H0. destruct H as ([ ] & _ & H). inv H. uncklr.
+  - econstructor; uncklr; eauto. congruence.
+  - inv H2. destruct H0 as ([ ] & _ & H0). inv H0. uncklr.
     eexists; split; constructor; eauto.
 Qed.
 
 End CORRECTNESS.
 
-Theorem transf_program_correct prog tprog:
+Theorem transf_program_correct prog tprog fn_stack_requirements:
   match_prog prog tprog ->
-  forward_simulation (cc_c ext) (cc_c ext) (CminorSel.semantics prog) (RTL.semantics tprog).
+  forward_simulation (cc_c ext) (cc_c ext) (CminorSel.semantics fn_stack_requirements prog) (RTL.semantics fn_stack_requirements tprog).
 Proof.
   fsim eapply forward_simulation_star_wf with (order := lt_state);
   intros; try destruct Hse.
