backend/RTLmachproof.v
@@ -1,7 +1,8 @@
 Require Import Coqlib Maps.
 Require Import AST Linking.
-Require Import Values Memory Globalenvs Events Smallstep.
+Require Import Values Memory Globalenvs Events Smallstep CKLR LanguageInterface Inject InjectFootprint.
 Require Import Op Registers RTL RTLmach.
+Require Tailcallproof.
 
 Definition transf_program (p: program) : program := p.
 
@@ -19,33 +20,16 @@ Variables fn_stack_requirements : ident -> Z.
 Variables prog: RTL.program.
 Variables tprog: program.
 Hypothesis TRANSL: match_prog prog tprog.
-Let ge := Genv.globalenv prog.
-Let tge := Genv.globalenv tprog.
+Variable w: world inj.
+Variable se: Genv.symtbl.
+Variable tse: Genv.symtbl.
+Let ge : RTL.genv := Genv.globalenv se prog.
+Let tge: genv := Genv.globalenv tse tprog.
+
+Hypothesis GE: match_stbls inj w se tse.
 
 Lemma prog_eq : prog = tprog.
 Proof. auto. Qed.
-
-Lemma genv_eq : ge = tge.
-Proof.
-  unfold match_prog in TRANSL. unfold ge.
-  unfold tge. congruence.
-Qed.
-
-Lemma find_function_translated:
-  forall ros rs rs' f,
-  find_function ge ros rs = Some f ->
-  regs_lessdef rs rs' ->
-  find_function ge ros rs' = Some f.
-Proof.
-  intros until f; destruct ros; simpl.
-  intros.
-  assert (rs'#r = rs#r).
-    exploit Genv.find_funct_inv; eauto. intros [b EQ].
-    generalize (H0 r). rewrite EQ. intro LD. inv LD. auto.
-  rewrite H1. auto.
-  destruct (Genv.find_symbol ge i); intros. auto.
-  discriminate.
-Qed.
 
 Lemma find_function_id_preserved:
   forall ros rs rs' id,
@@ -59,30 +43,73 @@ Proof.
   auto.
 Qed.
 
+Lemma functions_translated (j: meminj):
+  Genv.match_stbls j se tse ->
+  forall (v tv: val) (f: RTL.fundef),
+  Val.inject j v tv -> Genv.find_funct ge v = Some f ->
+  Genv.find_funct tge tv = Some f.
+Proof.
+  intros.
+  exploit Genv.find_funct_inv. eauto. intros [b EQ]. subst v. inv H0. rewrite Ptrofs.add_zero_l.
+  rewrite Genv.find_funct_find_funct_ptr in H1. unfold Genv.find_funct_ptr in H1.
+  destruct Genv.find_def as [[|]|] eqn:Hf; try congruence. inv H1.
+  exploit @Genv.globalenvs_match. red. intuition idtac.
+    instantiate (1 := prog). instantiate (2 := fun x y => x = y). instantiate (2 := fun x y z => y = z).
+    generalize (prog_defs prog). induction l; constructor; auto.
+    red. split. auto. destruct (snd a); econstructor; auto. reflexivity.
+    destruct v. constructor. auto. eauto.
+  intros MGE.
+  unfold Genv.find_def in Hf.
+  assert (sup_In b (Genv.genv_sup ge)) by eauto using Genv.genv_defs_range.
+  edestruct Genv.mge_dom; eauto. simpl in Hf.
+  pose proof (Genv.mge_defs MGE b H1). inv H2. congruence.
+  rewrite Hf in H3. inv H3. inv H6.
+  unfold Genv.find_funct, Genv.find_funct_ptr, Genv.find_def.
+  rewrite H1 in H4. inv H4. destr. 2:unfold Ptrofs.zero in n; congruence.
+  simpl. rewrite <- TRANSL, <- H5. auto.
+  Unshelve. exact tt.
+Qed.
+
+Lemma symbols_preserved:
+  forall j id ofs,
+  Genv.match_stbls j se tse ->
+  Val.inject j (Genv.symbol_address se id ofs) (Genv.symbol_address tse id ofs).
+Proof.
+  intros.
+  unfold Genv.symbol_address.
+  destruct (Genv.find_symbol se id) as [b|] eqn:FS; auto.
+  edestruct @Genv.find_symbol_match as (b' & Hb' & H'); eauto.
+  rewrite H'. econstructor; eauto. rewrite Ptrofs.add_zero. auto.
+Qed.
+
+
+Lemma ros_address_translated:
+  forall j ros rs rs',
+  regset_inject j rs rs' ->
+  Genv.match_stbls j se tse ->
+  Val.inject j (ros_address se ros rs) (ros_address tse ros rs').
+Proof.
+  intros. unfold ros_address, Genv.find_funct. destruct ros; auto.
+  apply symbols_preserved. auto.
+Qed.
+
 Lemma lessdef_list_refl : forall s,
     Val.lessdef_list s s.
 Proof.
   induction s; eauto.
 Qed.
 
-Inductive match_stackadt : Memory.stackadt -> Memory.stackadt -> Prop :=
-  |match_stackadt_nil : match_stackadt nil nil
-  |match_stackadt_cons : forall s1 s2 (t1:Memory.stage) (t1':Memory.stage) (frame:Memory.frame),
-     match_stackadt s1 s2 ->
+Inductive match_stackadt : nat -> Memory.stackadt -> Memory.stackadt -> Prop :=
+  | match_stackadt_nil: forall a1 a2
+      (IHsize: stack_size a1 >= stack_size a2),
+      match_stackadt 0 a1 a2
+  | match_stackadt_cons: forall n s1 s2 t1 t1' frame,
+     match_stackadt n s1 s2 ->
      t1 = frame::t1' ->
-     match_stackadt (t1::s1) ((frame::nil)::s2).
+     match_stackadt (S n) (t1::s1) ((frame::nil)::s2).
 
-Lemma match_stackadt_nonempty : forall s1 s2,
-    match_stackadt s1 s2 ->
-    s1 = nil <-> s2 = nil.
-Proof.
-  intros. inv H.
-  - reflexivity.
-  - split; congruence.
-Qed.
-
-Lemma match_stackadt_size : forall s1 s2,
-    match_stackadt s1 s2 ->
+Lemma match_stackadt_size : forall n s1 s2,
+    match_stackadt n s1 s2 ->
     Memory.stack_size s2 <= Memory.stack_size s1.
 Proof.
   intros. induction H.
@@ -92,47 +119,88 @@ Proof.
     lia.
 Qed.
 
-Lemma eval_builtin_arg_memiff:
-  forall sp rs m m0 args vargs,
-    eval_builtin_arg ge (fun r: positive => rs # r) sp m args vargs ->
-    Mem.iff m m0 ->
-    eval_builtin_arg ge (fun r: positive => rs # r) sp m0 args vargs.
+Inductive match_stackframes (j: meminj):
+  nat -> list nat -> list stackframe -> list stackframe -> Prop :=
+  | match_stackframes_nil:
+      meminj_preserves_globals ge j ->
+      meminj_global j ->
+      match_stackframes j 0 nil nil nil
+  | match_stackframes_normal: forall n l stk stk' res sp sp' pc rs rs' f,
+      match_stackframes j n l stk stk' ->
+      regset_inject j rs rs' ->
+      j sp = Some (sp',0) ->
+      match_stackframes j 0 ((S n)::l)
+        (Stackframe res f (Vptr sp Ptrofs.zero) pc rs :: stk)
+        (Stackframe res f (Vptr sp' Ptrofs.zero) pc rs' :: stk').
+
+Lemma match_stackframes_global : forall j n l stk stk',
+    match_stackframes j n l stk stk' ->
+    meminj_preserves_globals ge j /\ meminj_global j.
 Proof.
-  intros. induction H; constructor; eauto.
-  erewrite <- Mem.loadv_iff; eauto.
-  erewrite <- Mem.loadv_iff; eauto.
+  intros. induction H; auto.
 Qed.
 
-Lemma eval_builtin_args_memiff:
-  forall (sp : val) (rs : Regmap.t val) (m m0 : mem) (args : list (builtin_arg reg))
-    (vargs : list val) (H3 : eval_builtin_args ge (fun r : positive => rs # r) sp m args vargs)
-    (H7 : Mem.iff m m0),
-    eval_builtin_args ge (fun r : positive => rs # r) sp m0 args vargs.
+Lemma match_stackframes_incr : forall j j' stk stk' n l,
+    match_stackframes j n l stk stk' ->
+    inject_incr j j' ->
+    incr_without_glob j j' ->
+    match_stackframes j' n l stk stk'.
 Proof.
-  intros sp rs m m0 args vargs H3 H7.
-  unfold eval_builtin_args in *.
-  induction H3; constructor; auto.
-  eapply eval_builtin_arg_memiff; eauto.
+  intros.
+  induction H; constructor; auto.
+  - inversion H. inv H4.
+    split. eauto.
+    split. intros.
+    apply Genv.find_var_info_iff in H4 as A.
+    apply Genv.genv_info_range in A.
+    (* apply Genv.genv_defs_range in A. *)
+    apply Genv.genv_sup_glob in A. destruct A. subst. eauto.
+    intros.
+    destruct (j b1) eqn:?.
+    + destruct p. apply H0 in Heqo as H8. rewrite H7 in H8.
+      inv H8.
+      exploit H6. eauto. eauto. auto.
+    + exploit H1; eauto.
+    apply Genv.find_var_info_iff in H4 as A. apply Genv.genv_info_range in A.
+    apply Genv.genv_sup_glob in A. destruct A. subst.
+    intros [A B]. inv B.
+  - unfold meminj_global in *. intros.
+    destruct (j (Global id)) eqn:?. destruct p.
+    apply H0 in Heqo as H4. rewrite H3 in H4. inv H4.
+    apply H2 in Heqo. inv Heqo. auto.
+    exploit H1; eauto. intros [A B]. inv A.
+  - eapply regset_inject_incr; eauto.
 Qed.
 
 Inductive match_states: RTL.state -> RTL.state -> Prop :=
-  | match_regular_states: forall stk f sp pc rs m m',
-        Mem.iff m m' ->
-        match_stackadt (Mem.astack(Mem.support m)) (Mem.astack(Mem.support m'))->
-      match_states (State stk f sp pc rs m)
-                   (State stk f sp pc rs m')
-  | match_callstates: forall stk f args m sz m' hd tl,
-        Mem.iff m m' ->
-        Mem.astack(Mem.support m) = hd :: tl ->
-        match_stackadt tl (Mem.astack(Mem.support m')) ->
-      match_states (Callstate stk f args m sz)
-                   (Callstate stk f args m' sz)
-  | match_returnstates: forall stk v  m m' hd tl,
-        Mem.iff m m' ->
-        Mem.astack(Mem.support m) = hd :: tl ->
-        match_stackadt tl (Mem.astack(Mem.support m')) ->
-      match_states (Returnstate stk v m)
-                   (Returnstate stk v m').
+  | match_regular_states: forall j f s s' sp sp' pc rs rs' m m' n l
+        (STACKS: match_stackframes j n l s s')
+        (ASTK: match_stackadt (S (length s)) (Mem.astack (Mem.support m)) (Mem.astack (Mem.support m')))
+        (RINJ: regset_inject j rs rs')
+        (MINJ: Mem.inject j m m')
+        (SP: j sp = Some (sp', 0))
+        (INCR: inj_incr w (injw j (Mem.support m) (Mem.support m'))),
+      match_states (State s f (Vptr sp Ptrofs.zero) pc rs m)
+                   (State s' f (Vptr sp' Ptrofs.zero) pc rs' m')
+  | match_callstates: forall j s s' vf vf' args args' m m' id hd tl n l
+        (STACKS: match_stackframes j n l s s')
+        (FINJ: Val.inject j vf vf')
+        (AINJ: Val.inject_list j args args')
+        (MINJ: Mem.inject j m m')
+        (Heqastk: Mem.astack (Mem.support m) = hd :: tl)
+        (ASTK: match_stackadt (length s) tl (Mem.astack (Mem.support m')))
+        (INCR: inj_incr w (injw j (Mem.support m) (Mem.support m'))),
+      match_states (Callstate s vf args m id)
+                   (Callstate s' vf' args' m' id)
+  | match_returnstates: forall j s s' v v' m m' hd tl n l
+        (STACKS: match_stackframes j n l s s')
+        (VINJ: Val.inject j v v')
+        (MINJ: Mem.inject j m m')
+        (Heqastk: Mem.astack (Mem.support m) = hd :: tl)
+        (ASTK: match_stackadt (length s) tl (Mem.astack (Mem.support m')))
+        (INCR: inj_incr w (injw j (Mem.support m) (Mem.support m'))),
+      match_states (Returnstate s v m)
+                   (Returnstate s' v' m').
 
 Lemma step_simulation:
   forall S1 t S2, RTL.step fn_stack_requirements ge S1 t S2 ->
@@ -140,160 +208,361 @@ Lemma step_simulation:
   exists S2', step fn_stack_requirements tge S1' t S2' /\ match_states S2 S2'.
 Proof.
   intros. inv H; inv H0.
-  - econstructor; eauto. split.
-    econstructor; eauto.
-    econstructor; eauto.
-  - econstructor; eauto. split.
-    eapply exec_Iop; eauto. rewrite <- genv_eq.
-    eapply eval_operation_memiff; eauto.
-    econstructor; eauto.
-  - econstructor; eauto. split.
-    rewrite <- genv_eq.
-    eapply exec_Iload; eauto.
-    erewrite <- Mem.loadv_iff; eauto.
-    econstructor; eauto.
-  - exploit Mem.storev_iff; eauto.
-    intros (m2' & H3' & IFF').
+
+  - (* nop *)
     econstructor; eauto. split.
-    rewrite <- genv_eq.
-    eapply exec_Istore; eauto.
     econstructor; eauto.
-    rewrite <- (Mem.support_storev _ _ _ _ _ H3).
-    rewrite <- (Mem.support_storev _ _ _ _ _ H3').
-    auto.
-  - econstructor; eauto. split.
-    rewrite <- genv_eq.
-    eapply exec_Icall; eauto.
     econstructor; eauto.
-    eapply Mem.push_stage_left_iff; eauto.
-    simpl. reflexivity.
-  - edestruct Mem.free_parallel_iff as [m1' []]; eauto.
-    inv H13. 
-    erewrite <- Mem.support_free in H7; eauto. congruence.
-    assert ({m2':mem|Mem.pop_stage m1'= Some m2'}).
-      apply Mem.nonempty_pop_stage.
-      erewrite Mem.support_free. 2: eauto. congruence.
-    destruct X as [m'2 POP].
-    apply Mem.astack_pop_stage in POP as STKm2'.
-    destruct STKm2' as [hd STKm2'].
+
+  - (* op *)
+    assert (Val.inject_list j (rs##args) (rs'##args)). apply regs_inject; auto.
+    exploit eval_operation_inject; eauto.
+    eapply CKLR.match_stbls_acc in GE; eauto. apply GE.
+    intros [v' [EVAL' VINJ]].
+    rewrite eval_shift_stack_operation in EVAL'. eauto.
     econstructor; eauto. split.
-    rewrite <- genv_eq.
-    eapply exec_Itailcall; eauto.
-    econstructor; eauto.
-    eapply Mem.pop_stage_right_iff; eauto.
-    erewrite Mem.support_free. 2: eauto. eauto.
-    erewrite <- Mem.support_free in H7; eauto.
-    congruence.
-  - exploit Mem.push_stage_left_iff; eauto. intro.
-    exploit external_call_mem_iff; eauto. intros (m'1 & EXT &IFF').
+    eapply exec_Iop; eauto.
+    econstructor; eauto. apply set_reg_inject; auto.
+
+  - (* load *)
+    assert (Val.inject_list j (rs##args) (rs'##args)). apply regs_inject; auto.
+    exploit eval_addressing_inject; eauto. eapply CKLR.match_stbls_acc in GE; eauto. apply GE.
+    intros [a' [ADDR' AINJ]].
+    exploit Mem.loadv_inject; eauto.
+    intros [v' [LOAD' VINJ]].
     econstructor; eauto. split.
-    rewrite <- genv_eq.
-    econstructor; eauto.
-    eapply eval_builtin_args_memiff; eauto.
-    econstructor; eauto.
-    eapply Mem.pop_stage_left_iff; eauto.
-    rewrite <- (external_call_astack _ _ _ _ _ _ _ EXT).
-    apply Mem.astack_pop_stage in H4. destruct H4.
-    rewrite <- (external_call_astack _ _ _ _ _ _ _ H3) in H0.
-    simpl in H0. inv H0. auto.
-  - econstructor; eauto. split.
-    rewrite <- genv_eq.
+    eapply exec_Iload with (a := a'). eauto.
+    rewrite eval_shift_stack_addressing in ADDR'. auto. eauto.
+    econstructor; eauto. apply set_reg_inject; auto.
+
+  - (* store *)
+    assert (Val.inject_list j (rs##args) (rs'##args)). apply regs_inject; auto.
+    exploit eval_addressing_inject; eauto.
+    eapply CKLR.match_stbls_acc in GE; eauto. apply GE.
+    intros [a' [ADDR' AINJ]].
+    exploit Mem.storev_mapped_inject. 2: eexact H3. eauto. eauto. apply RINJ.
+    intros [m'1 [STORE' MINJ']].
+    eexists. split.
+    eapply exec_Istore with (a := a'). eauto.
+    rewrite eval_shift_stack_addressing in ADDR'. rewrite <- ADDR'. auto. eauto.
+    destruct a; simpl in H1; try discriminate.
+    apply Mem.support_store in H3 as S.
+    apply Mem.support_storev in STORE' as S'.
+    econstructor; eauto. congruence.
+    rewrite S, <- S'. auto.
+
+  - (* call *)
+    apply match_stackframes_global in STACKS as GLOB. destruct GLOB.
+    exploit functions_translated.
+    eapply CKLR.match_stbls_acc in GE; eauto. apply GE.
+    2:eauto. apply ros_address_translated; eauto.
+    eapply CKLR.match_stbls_acc in GE; eauto. apply GE.
+    intro FIND'.
+    econstructor; eauto. split.
+    eapply exec_Icall; eauto. eapply Tailcallproof.ros_is_ident_translated; eauto.
+    econstructor. constructor; eauto.
+    apply ros_address_translated; eauto.
+    eapply CKLR.match_stbls_acc in GE; eauto. apply GE.
+    apply regs_inject; auto. eapply Mem.push_stage_left_inject; eauto.
+    simpl. eauto. auto. destruct w. inv INCR. constructor; auto.
+
+  - (* tailcall *)
+    apply match_stackframes_global in STACKS as GLOB. destruct GLOB.
+    exploit functions_translated.
+    eapply CKLR.match_stbls_acc in GE; eauto. apply GE.
+    2:eauto. apply ros_address_translated; eauto.
+    eapply CKLR.match_stbls_acc in GE; eauto. apply GE.
+    intro FIND'.
+    exploit Mem.free_parallel_inject; eauto. intros [m'1 [FREE INJ]].
+    apply Mem.support_free in H5 as SF. apply Mem.support_free in FREE as SF'.
+    pose proof Mem.nonempty_pop_stage m'1. destruct X as (m'2 & POP).
+    inv ASTK. congruence.
+    destruct (Mem.astack (Mem.support m')) eqn:CONS. congruence.
+    eexists. split.
+    eapply exec_Itailcall; eauto. eapply Tailcallproof.ros_is_ident_translated; eauto.
+    rewrite ! Z.add_0_r in FREE. eauto.
+    econstructor. eauto.
+    apply ros_address_translated; eauto.
+    eapply CKLR.match_stbls_acc in GE; eauto. apply GE.
+    apply regs_inject. auto.
+    eapply Mem.pop_stage_right_inject; eauto.
+    eauto.
+    inv ASTK. rewrite <- SF, CONS in H7. inv H7.
+    apply Mem.astack_pop_stage in POP as [hd EQ].
+    rewrite <- SF', EQ in H8. inv H8. auto.
+    rewrite SF. inv INCR. constructor; auto.
+    red. intros. rewrite <- Mem.support_pop_stage_1. 2:eauto.
+    rewrite SF'. auto.
+
+  - (* builtin *)
+    apply match_stackframes_global in STACKS as GLOB. destruct GLOB.
+    exploit Tailcallproof.eval_builtin_args_inject; eauto.
+      eapply CKLR.match_stbls_acc in GE; eauto. apply GE.
+    intros (vargs' & P & Q).
+    exploit Mem.push_stage_inject; eauto. intro.
+    exploit external_call_mem_inject'. 2:eauto.
+      eapply CKLR.match_stbls_acc in GE; eauto. apply GE.
+      apply Mem.push_stage_left_inject. eauto. eauto. simpl.
+    intros [f' [v' [m'1 [A [B [C [D [E [F [G [I [J K]]]]]]]]]]]].
+    exploit Mem.pop_stage_left_inject; eauto. intros EXT'.
+    eexists. split.
+    eapply exec_Ibuiltin; eauto.
+    econstructor. 4:eauto. all:eauto.
+    eapply match_stackframes_incr; eauto.
+    apply Mem.astack_pop_stage in H4 as [hd EQ]. rewrite EQ in F. inv F. congruence.
+    apply set_res_inject; eauto. eapply regset_inject_incr; eauto.
+    etransitivity. eauto. constructor; auto; red; intros.
+    apply Mem.unchanged_on_support in D. apply D in H6.
+    rewrite Mem.support_pop_stage_1 in H6; eauto.
+    apply Mem.unchanged_on_support in E. apply E in H6. auto.
+
+  - (* cond *)
+    econstructor; eauto. split.
     eapply exec_Icond; eauto.
-    erewrite <- eval_condition_memiff; eauto.
+    apply eval_condition_inject with j (rs##args) m; auto. apply regs_inject; auto. eauto.
     econstructor; eauto.
-  - econstructor; eauto. split.
-    rewrite <- genv_eq.
+
+  - (* jumptable *)
+    econstructor; eauto. split.
     eapply exec_Ijumptable; eauto.
+    generalize (RINJ arg). rewrite H2. intro. inv H. auto.
     econstructor; eauto.
-  - edestruct Mem.free_parallel_iff as [m'1[]]; eauto.
-    apply Mem.support_free in H2 as SFREE.
-    apply Mem.support_free in H as SFREE'.
-    inv H11. congruence.
-    assert ({m'2:mem|Mem.pop_stage m'1= Some m'2}).
-      apply Mem.nonempty_pop_stage. congruence.
-    destruct X as [m'2 POP].
-    econstructor; eauto. split.
+
+  - (* return *)
+    exploit Mem.free_parallel_inject; eauto. intros [m'1 [FREE INJ]].
+    apply Mem.support_free in H2 as SF. apply Mem.support_free in FREE as SF'.
+    pose proof Mem.nonempty_pop_stage m'1 as [m'2 POP].
+      rewrite SF'. inv ASTK. congruence.
+    eexists. split.
     eapply exec_Ireturn; eauto.
-    econstructor; eauto.
-    eapply Mem.pop_stage_right_iff; eauto.
-    rewrite SFREE. eauto.
-    apply Mem.astack_pop_stage in POP. destruct POP. congruence.
-  - edestruct Mem.alloc_parallel_iff as [m'2 []]; eauto.
-    apply Mem.support_alloc in H1 as SAL.
-    apply Mem.support_alloc in H as SAL'.
-    exploit Mem.push_stage_right_iff. apply H0. intro.
-    apply Mem.astack_record_frame in H2 as ASTK.
-    apply Mem.record_frame_size1 in H2 as SIZE. simpl in SIZE.
-    destruct ASTK as (hd' & tl' & ASTKm' & ASTKm''). rewrite ASTKm' in SIZE.
-    rewrite SAL in ASTKm'.
-    simpl in ASTKm'.
-    rewrite H9 in ASTKm'. inv ASTKm'.
-    assert ({m'3:mem|Mem.record_frame (Mem.push_stage m'2) (Memory.mk_frame (Stack 1%positive) (fn_stack_requirements id)) = Some m'3}).
-      apply Mem.request_record_frame. simpl. congruence.
-      simpl. rewrite SAL'. simpl.
-      apply match_stackadt_size in H10. simpl in *.
-      generalize (size_of_all_frames_pos hd'). lia.
-    destruct X as [m'3 RECORD].
-    econstructor; eauto. split.
-    econstructor; eauto.
-    econstructor; eauto.
-    eapply Mem.record_frame_safe_iff; eauto.
-    apply Mem.astack_record_frame in RECORD as ASTK.
-    destruct ASTK as (hd''&tl''&STKm'1&STKm'2).
-    rewrite STKm'2. simpl in STKm'1. inv STKm'1.
-    rewrite ASTKm''. econstructor. 2:eauto.
-    rewrite SAL'. unfold sup_incr. simpl. auto.
-  - exploit external_call_mem_iff; eauto.
-    intros (m2' & H1'& IFF).
-    econstructor; eauto. split.
-    rewrite <- genv_eq.
-    econstructor; eauto.
-    econstructor; eauto.
-    rewrite <- (external_call_astack _ _ _ _ _ _ _ H1). eauto.
-    rewrite <- (external_call_astack _ _ _ _ _ _ _ H1'). eauto.
-  - apply Mem.stack_pop_stage in H1 as H1'. destruct H1'.
-    econstructor; eauto. split.
-    econstructor; eauto.
-    econstructor; eauto.
-    eapply Mem.pop_stage_left_iff; eauto.
-    apply Mem.astack_pop_stage in H1. destruct H1. rewrite H in H6. inv H6.
+    rewrite ! Z.add_0_r in FREE. eauto.
+    destruct (Mem.astack (Mem.support m')) eqn:Heqm'. congruence.
+    econstructor. eauto.
+    inv ASTK. apply Mem.astack_pop_stage in POP as [hd EQ].
+    rewrite SF' in EQ. rewrite EQ in H4. inv H4.
+    destruct or; simpl. apply RINJ. constructor.
+    exploit Mem.pop_stage_right_inject; eauto.
+    eauto.
+    inv ASTK. clear H3.
+    rewrite SF, <- H0 in Heqm'. inv Heqm'.
+    apply Mem.astack_pop_stage in POP as POPRES. destruct POPRES as [hd POP'].
+    congruence.
+    inv INCR. constructor; auto.
+    red. intros. rewrite SF. auto.
+    red. intros. rewrite <- Mem.support_pop_stage_1. rewrite SF'. auto. auto.
+
+  - (* internal call *)
+    exploit functions_translated; eauto.
+    eapply CKLR.match_stbls_acc in GE; eauto. apply GE.
+    intro FIND'.
+    exploit Mem.alloc_parallel_inject; eauto.
+      instantiate (1 := 0). lia.
+      instantiate (1 := fn_stacksize f). lia.
+    intros (f' & m'1 & b2 & ALLOC & INJ' & INCR' & GLOB' & TSP & INC).
+    apply Mem.astack_record_frame in H2 as ASTK1.
+    apply Mem.record_frame_size1 in H2 as SIZE.
+    destruct ASTK1 as (hd' & tl' & ASTKm' & ASTKm''). rewrite ASTKm' in SIZE.
+    erewrite <- Mem.astack_alloc in Heqastk; eauto. rewrite ASTKm' in Heqastk. inv Heqastk.
+    exploit Mem.record_frame_parallel_inject. 2:eauto.
+      apply Mem.push_stage_right_inject. eauto.
+      simpl. congruence.
+      simpl. erewrite Mem.astack_alloc; eauto. rewrite ASTKm'.
+      apply match_stackadt_size in ASTK.
+      simpl. pose proof size_of_all_frames_pos hd. lia.
+    intros (m'2 & RECORD & INJ'').
+    apply Mem.astack_record_frame in RECORD as ASTK2.
+    destruct ASTK2 as (hd' & tl' & ASTKm'1 & ASTKm'2).
+    simpl in ASTKm'1. inv ASTKm'1.
+    econstructor; split.
+    simpl. eapply exec_function_internal; eauto.
+    econstructor.
+    eapply match_stackframes_incr; eauto.
+    rewrite ASTKm'2, ASTKm''. econstructor. erewrite Mem.astack_alloc; eauto. eauto.
+    apply Tailcallproof.init_regs_inject.
+    eapply val_inject_list_incr; eauto. auto. auto.
+    assert (SPS: b2 = fresh_block (Mem.support m'0)) by (eapply Mem.alloc_result; eauto).
+    eapply Tailcallproof.mit_incr_invariant. apply INCR'.
     auto.
+    instantiate (1 := (Mem.support m'0)).
+    inv INCR. simpl.
+    intros. destruct (eq_block b1 stk).
+      subst b1. rewrite TSP in H; inv H.
+        apply Mem.alloc_result in H1. subst.
+        exfalso. destruct H0; eapply freshness; eauto.
+      rewrite INC in H; auto.
+    inv INCR. simpl. auto.
+    eauto.
+    red. intros. rewrite <- Mem.support_record_frame_1. 2:eauto.
+    apply Mem.support_alloc in H1. rewrite H1.
+    apply Mem.mem_incr_2. auto.
+    red. intros. rewrite <- Mem.support_record_frame_1. 2:eauto.
+    erewrite Mem.support_push_stage.
+    apply Mem.support_alloc in ALLOC. rewrite ALLOC.
+    apply Mem.mem_incr_2. auto. auto.
+
+  - (* external call *)
+    exploit functions_translated; eauto.
+    eapply CKLR.match_stbls_acc in GE; eauto. apply GE.
+    intro FIND'.
+    exploit external_call_mem_inject'; eauto.
+    eapply CKLR.match_stbls_acc in GE; eauto. apply GE.
+    intros (f' & res' & m2' & A & B & C & D & E & F & G & I & J & K).
+    exists (Returnstate s' res' m2'); split.
+    simpl. econstructor; eauto.
+    econstructor. eapply match_stackframes_incr; eauto.
+    auto. auto. rewrite <- F. eauto. rewrite <- G. auto.
+    etransitivity; eauto.
+    apply Mem.unchanged_on_support in D.
+    apply Mem.unchanged_on_support in E.
+    constructor; auto.
+
+  - (* returnstate *)
+    inv STACKS.
+    econstructor; split.
+    apply exec_return. econstructor; eauto.
+    apply Mem.astack_pop_stage in H1. destruct H1.
+    rewrite H in Heqastk. inv Heqastk. simpl in ASTK. auto.
+    apply set_reg_inject; auto.
+    eapply Mem.pop_stage_left_inject; eauto.
+    inv INCR. constructor; auto; red; intros.
+    erewrite <- Mem.support_pop_stage_1. 2:eauto. auto.
 Qed.
 
 Lemma transf_initial_states:
-  forall S1, RTL.initial_state prog S1 ->
-  exists S2, initial_state tprog S2 /\ match_states S1 S2.
+  forall q1 q2 st1, match_query (cc_c inj) w q1 q2 -> RTL.initial_state ge q1 st1 ->
+  exists st2, initial_state tge q2 st2 /\ match_states st1 st2.
 Proof.
-  intros. inv TRANSL. inv H.
-  exists (Callstate nil f nil m1 (prog_main tprog)).
-  split.
+  intros. destruct H. inv H0.
+  exploit functions_translated; eauto. apply GE. intro FIND.
+  exists (Callstate nil vf2 vargs2 m2 id); split.
   econstructor; eauto.
-  econstructor; eauto.
-  eapply Mem.push_stage_left_iff. apply Mem.iff_refl.
-  simpl. reflexivity. erewrite Mem.astack_alloc; eauto.
-  apply Genv.init_mem_astack in H0. rewrite H0.
-  constructor.
+  inv H. inv H2. apply INJG in H5 as [ ]. subst. auto using Ptrofs.add_zero_l.
+  inv H2. inv ASTK.
+  econstructor; eauto. constructor.
+  red. split; [|split]; intros; simpl.
+
+  inv GE. inv inj_stbls_match.
+  apply Genv.genv_symb_range in H2 as ?.
+  apply mge_dom in H4 as [b' ?].
+  eapply mge_symb in H4 as ?. destruct H5. specialize (H5 H2). clear H6.
+  apply Genv.genv_vars_eq in H2. apply Genv.genv_vars_eq in H5. subst. auto.
+
+  inv GE. inv inj_stbls_match.
+  rewrite Genv.find_var_info_iff in H2.
+  apply Genv.genv_info_range in H2 as ?.
+  apply Genv.genv_sup_glob in H4 as ?. destruct H5 as (id' & ?). subst.
+  apply mge_dom in H4 as [b' ?].
+  inv H2. apply INJG in H4 as ?. destruct H2. subst. rewrite H4. auto.
+
+  inv GE. inv inj_stbls_match.
+  rewrite Genv.find_var_info_iff in H2.
+  apply Genv.genv_info_range in H2 as ?.
+  apply Genv.genv_sup_glob in H4 as ?. destruct H6 as (id' & ?). subst.
+  apply mge_dom in H4 as [b' ?].
+  apply INJG in H4 as ?. destruct H6. subst. simpl in *.
+  apply mge_separated in H5 as ?.
+  setoid_rewrite mge_info in H2. 2:eauto.
+  apply Genv.genv_info_range in H2. rewrite <- H6 in H2.
+  apply Genv.genv_sup_glob in H2 as [id'' ?]. subst.
+  apply INJG in H5 as [ ]. subst. auto.
+
+  subst. auto.
+
+  subst. simpl. apply Mem.push_stage_left_inject. auto.
+
+  simpl. auto.
+
+  econstructor; simpl; auto.
+
+  subst. constructor; simpl in *; auto.
+  all:red; intros. congruence.
+  congruence.
+  all:
+    (erewrite <- Mem.support_push_stage; [|eauto]);
+    (rewrite <- Mem.support_push_stage_1; [|eauto]);
+    auto.
 Qed.
 
 Lemma transf_final_states:
-  forall S1 S2 r, match_states S1 S2 -> RTL.final_state S1 r -> final_state S2 r.
+  forall st1 st2 r1, match_states st1 st2 -> RTL.final_state st1 r1 ->
+  exists r2, final_state st2 r2 /\ match_reply (cc_c inj) w r1 r2.
 Proof.
-  intros. inv H0. inv H. constructor.
+  intros. inv H0. inv H. inv STACKS. inv INCR.
+  eexists; split.
+  - constructor.
+  - econstructor.
+    split; constructor.
+    4:red; intros; rewrite <- Mem.support_pop_stage_1; eauto. all:eauto.
+    constructor; auto.
+    inv ASTK. constructor.
+    apply Mem.astack_pop_stage in H1 as [ ]. rewrite H1 in Heqastk. inv Heqastk. auto.
+    eapply Mem.pop_stage_left_inject; eauto.
 Qed.
 
-
-Theorem transf_program_correct:
-  forward_simulation (RTL.semantics fn_stack_requirements prog)
-                     (RTLmach.semantics fn_stack_requirements tprog).
+Lemma transf_external_states:
+  forall st1 st2 q1, match_states st1 st2 -> RTL.at_external ge st1 q1 ->
+  exists wx q2, at_external tge st2 q2 /\ match_query (cc_c injp) wx q1 q2 /\ match_senv (cc_c injp) wx se tse /\
+  forall r1 r2 st1', match_reply (cc_c injp) wx r1 r2 -> RTL.after_external st1 r1 st1' ->
+  exists st2', after_external st2 r2 st2' /\ match_states st1' st2'.
 Proof.
-  eapply forward_simulation_step.
-  rewrite prog_eq. auto.
-  eexact transf_initial_states.
-  eexact transf_final_states.
-  exact step_simulation.
+  intros st1 st2 q1 Hst Hq1. destruct Hq1. inv Hst.
+  assert (GE0: Genv.match_stbls j se tse). {
+    inv GE. inv INCR. eapply Genv.match_stbls_incr; eauto. simpl.
+    split; intro; (exploit DISJOINT; eauto); intros [ ].
+    apply inj_stbls_next_l in H2. auto.
+    apply inj_stbls_next_r in H2. auto.
+  }
+  assert (VF: vf' = Vptr (Global id) Ptrofs.zero). {
+    inv FINJ. rewrite Ptrofs.add_zero_l.
+    apply match_stackframes_global in STACKS as [ ]. apply H1 in H2 as [ ]. subst. auto.
+  }
+  exploit functions_translated; eauto.
+  intro FIND'.
+  exists (injpw j m m' MINJ). eexists. intuition idtac.
+  - econstructor; eauto.
+  - constructor; simpl; auto. constructor; auto.
+    apply match_stackframes_global in STACKS as [ ]. auto.
+    constructor. apply match_stackadt_size in ASTK. rewrite Heqastk. simpl.
+    pose proof size_of_all_frames_pos hd. lia.
+    congruence.
+  - inv GE. inv INCR. simpl in *. constructor; simpl. auto.
+    red. red in inj_stbls_next_l. auto.
+    red. red in inj_stbls_next_r. auto.
+  - inv H2. destruct H1 as (w' & ACC & CR). inv CR.
+    destruct w'. simpl in ACC, H3, H5. inv H5.
+    (* destruct H0 as ([ ] & [ ] & H0). inv H0. CKLR.uncklr. *)
+    exists (Returnstate s' vres2 m2'). split.
+    constructor; auto.
+    econstructor.
+    inv ACC. eapply match_stackframes_incr; eauto.
+    auto. auto.
+    inv ACC. rewrite <- ASTK1. eauto.
+    inv ACC. rewrite <- ASTK2. auto.
+    etransitivity. eauto.
+    inv ACC. econstructor; eauto.
+    inv UNMAPPED. eauto. inv UNREACH. eauto.
 Qed.
 
 End PRESERVATION.
+
+Theorem transf_program_correct prog tprog fn_stack_requirements:
+  match_prog prog tprog ->
+  forward_simulation (cc_c injp) (cc_c inj) (RTL.semantics fn_stack_requirements prog) (RTLmach.semantics fn_stack_requirements tprog).
+Proof.
+  fsim eapply forward_simulation_step.
+  - inv MATCH. auto.
+  - intros q1 q2 Hq. destruct Hq. cbn in *. inv Hse. cbn in *.
+    eapply Genv.is_internal_transf; eauto.
+    instantiate (1 := id). red. red. inv MATCH. intuition.
+    generalize (prog_defs tprog). induction l; constructor; auto.
+    red. intuition. simpl. destruct b; econstructor; auto.
+    apply linkorder_refl. destruct v. econstructor. auto.
+    auto.
+  - eapply transf_initial_states; eauto.
+  - eapply transf_final_states; eauto.
+  - intros. eapply transf_external_states; eauto.
+  - eapply step_simulation; eauto.
+Qed.
 
 Instance TransfRTLmachLink : TransfLink match_prog.
 Proof.
